verified/subdir.mk
@@ -1,4 +1,4 @@
-DAFNYFLAGS = /timeLimit:80 /trace #/proc:*exceptionHandled*
+DAFNYFLAGS = /timeLimit:70 /trace 
 SPARTANFLAGS = #-assumeUpdates 1
 
 # top-level target
@@ -92,6 +92,10 @@ init_l2ptable_dep-sdfy = ARMdecls kom_utils allocate_page
 init_l2ptable_dep-dfy = ARMspartan kom_common.i pagedb.i smcapi.i
 $(dir)/init_l2ptable.verified: $(call mkdeps,init_l2ptable)
 
+map_secure_dep-sdfy = ARMdecls kom_utils allocate_page
+map_secure_dep-dfy = ARMspartan kom_common.i pagedb.i smcapi.i abstate.s entry.i
+$(dir)/map_secure.verified: $(call mkdeps,map_secure)
+
 enter_dep-sdfy = ARMdecls kom_utils
 enter_dep-dfy = ARMspartan kom_common.i pagedb.i smcapi.i abstate.s entry.i
 $(dir)/enter.verified: $(call mkdeps,enter)
@@ -101,6 +105,6 @@ resume_dep-dfy = ARMspartan kom_common.i pagedb.i smcapi.i abstate.s entry.i
 $(dir)/resume.verified: $(call mkdeps,resume)
 
 smc_handler_dep-sdfy = ARMdecls kom_utils init_addrspace init_dispatcher \
-    init_l2ptable enter resume
-smc_handler_dep-dfy = ARMspartan kom_common.i pagedb.i smcapi.i
+    init_l2ptable enter resume map_secure
+smc_handler_dep-dfy = ARMspartan kom_common.i pagedb.i smc api.i
 $(dir)/smc_handler.verified: $(call mkdeps,smc_handler)
